implement modulo operation for memory addresses
Before, when loading and storing to or from an adress, a natural number
was used. This simplified the semantics, but allowed reading and writing
to memory locations just after the allowed address range if a large word
needed to be read from or stored in multiple memory locations. The
original idea was that the caller needs to take care of this via eg.
alignment checks.

After the chat with Roberto yesterday, I implemented the modulo
operation on memory addresses directly in bir.

bir_expScript.sml
@@ -63,7 +63,7 @@ val bir_eval_ifthenelse_def = Define `
 val bir_eval_load_def = Define `
   (bir_eval_load (BVal_Mem ta tv mmap) (BVal_Imm a) en t =
      if ((type_of_bir_imm a) = ta) then
-        (case (bir_load_from_mem tv t mmap en (b2n a)) of
+        (case (bir_load_from_mem tv t ta mmap en (b2n a)) of
            NONE => BVal_Unknown
          | SOME i => BVal_Imm i)
      else BVal_Unknown) /\
@@ -72,7 +72,7 @@ val bir_eval_load_def = Define `
 val bir_eval_store_def = Define `
   (bir_eval_store (BVal_Mem ta tv mmap) (BVal_Imm a) en (BVal_Imm v) =
      if ((type_of_bir_imm a) = ta) then
-        (case (bir_store_in_mem tv v mmap en (b2n a)) of
+        (case (bir_store_in_mem tv ta v mmap en (b2n a)) of
            NONE => BVal_Unknown
          | SOME mmap' => BVal_Mem ta tv mmap')
      else BVal_Unknown) /\
@@ -223,7 +223,7 @@ ASM_SIMP_TAC std_ss [bir_load_from_mem_NO_ENDIAN]);
 
 val bir_eval_load_Unknown_REWRS5 = prove (
   ``!a en t i aty vty mmap en.
-      (bir_number_of_mem_splits vty t = NONE) ==>
+      (bir_number_of_mem_splits vty t aty = NONE) ==>
       (bir_eval_load (BVal_Mem aty vty mmap) (BVal_Imm i) en t = BVal_Unknown)``,
 
 SIMP_TAC std_ss [bir_eval_load_def] >>
@@ -245,14 +245,20 @@ val bir_eval_load_SINGLE_REWR = store_thm ("bir_eval_load_SINGLE_REWR",
       ((if (type_of_bir_imm i = aty) then (BVal_Imm (n2bs (mmap (b2n i)) vty))
        else BVal_Unknown))``,
 
-SIMP_TAC arith_ss [bir_eval_load_def, bir_load_from_mem_SINGLE]);
+SIMP_TAC arith_ss [bir_eval_load_def, bir_load_from_mem_SINGLE] >>
+REPEAT STRIP_TAC >>
+COND_CASES_TAC >> ASM_REWRITE_TAC[] >>
+`bir_mem_addr aty (b2n i) = b2n i` suffices_by ASM_SIMP_TAC std_ss [] >>
+MATCH_MP_TAC bir_mem_addr_id >>
+METIS_TAC[b2n_lt]
+);
 
 
 val bir_eval_load_BASIC_REWR = store_thm ("bir_eval_load_BASIC_REWR",
   ``!a en t i aty vty ty mmap en.
       (bir_eval_load (BVal_Mem aty vty mmap) (BVal_Imm i) en ty) =
       (if type_of_bir_imm i = aty then
-        case bir_load_from_mem vty ty mmap en (b2n i) of
+        case bir_load_from_mem vty ty aty mmap en (b2n i) of
           NONE => BVal_Unknown
         | SOME i => BVal_Imm i
        else BVal_Unknown)``,
@@ -265,17 +271,22 @@ let
       (type_of_bir_imm a <> ta) ==>
       (bir_eval_load (BVal_Mem ta tv mmap) (BVal_Imm a) en tr = BVal_Unknown)) /\
       (!tr tv.
-      (tr <> tv) ==> (bir_number_of_mem_splits tv tr <> NONE) ==>
+      (tr <> tv) ==> (bir_number_of_mem_splits tv tr ta <> NONE) ==>
       (bir_eval_load (BVal_Mem ta tv mmap) (BVal_Imm i) BEnd_NoEndian tr = BVal_Unknown)) /\
       (!tr tv.
-      (bir_number_of_mem_splits tv tr = NONE) ==>
+      (bir_number_of_mem_splits tv tr ta = NONE) ==>
       (bir_eval_load (BVal_Mem ta tv mmap) (BVal_Imm i) en tr = BVal_Unknown))``,
    SIMP_TAC std_ss [bir_eval_load_Unknown_REWRS])
 
   val thm_prune1 = SIMP_RULE (std_ss ++ bir_imm_ss ++ DatatypeSimps.expand_type_quants_ss [``:bir_immtype_t``, ``:bir_imm_t``]) [bir_number_of_mem_splits_REWRS, type_of_bir_imm_def] thm_prune0
 
-  val thm_prune2 = SIMP_RULE std_ss [FORALL_AND_THM, GSYM CONJ_ASSOC] (GEN_ALL thm_prune1)
 
+  val (l1, l2) = partition (is_imp_only o concl) (CONJUNCTS thm_prune1)
+
+  val l1' = map (SIMP_RULE (list_ss++bir_imm_ss++DatatypeSimps.expand_type_quants_ss [``:bir_immtype_t``]) [bir_number_of_mem_splits_REWRS] o (Q.GEN `ta`)) l1
+
+  val thm_prune2 = SIMP_RULE std_ss [FORALL_AND_THM, GSYM CONJ_ASSOC] (GEN_ALL
+    (LIST_CONJ (l1' @ l2)))
 
   val thm0 = bir_eval_load_BASIC_REWR
 
@@ -288,7 +299,7 @@ let
      FORALL_AND_THM, b2n_MOD_2EXP, type_of_bir_imm_def, size_of_bir_immtype_def]
      thm2
 
-  val thm4 = REWRITE_RULE [b2n_def, GSYM CONJ_ASSOC] (CONJ thm3 thm_prune2)
+  val thm4 = REWRITE_RULE [b2n_def, bir_mem_addr_w2n_sizes, GSYM CONJ_ASSOC] (CONJ thm3 thm_prune2)
 in thm4
 end);
 
@@ -338,7 +349,7 @@ ASM_SIMP_TAC std_ss [bir_store_in_mem_NO_ENDIAN]);
 
 val bir_eval_store_Unknown_REWRS6 = prove (
   ``!a en v aty vty mmap en.
-      (bir_number_of_mem_splits vty (type_of_bir_imm v) = NONE) ==>
+      (bir_number_of_mem_splits vty (type_of_bir_imm v) aty = NONE) ==>
       (bir_eval_store (BVal_Mem aty vty mmap) a en (BVal_Imm v) = BVal_Unknown)``,
 
 Cases_on `a` >> SIMP_TAC std_ss [bir_eval_store_def, LET_DEF] >>
@@ -359,15 +370,18 @@ val bir_eval_store_SINGLE_REWR = store_thm ("bir_eval_store_SINGLE_REWR",
       (bir_eval_store (BVal_Mem aty vty mmap) (BVal_Imm i) en (BVal_Imm v) =
       (BVal_Mem aty vty ((b2n i =+ b2n v) mmap)))``,
 
-SIMP_TAC arith_ss [bir_eval_store_def, bir_store_in_mem_SINGLE]);
-
+SIMP_TAC arith_ss [bir_eval_store_def, bir_store_in_mem_SINGLE] >>
+REPEAT STRIP_TAC >>
+`bir_mem_addr (type_of_bir_imm i) (b2n i) = b2n i` suffices_by ASM_SIMP_TAC std_ss [] >>
+MATCH_MP_TAC bir_mem_addr_id >>
+METIS_TAC[b2n_lt]);
 
 
 val bir_eval_store_BASIC_REWR = store_thm ("bir_eval_store_BASIC_REWR",
   ``!a en t i aty v vty mmap en.
       (bir_eval_store (BVal_Mem aty vty mmap) (BVal_Imm i) en (BVal_Imm v) =
       (if type_of_bir_imm i = aty then
-         case bir_store_in_mem vty v mmap en (b2n i) of
+         case bir_store_in_mem vty aty v mmap en (b2n i) of
            NONE => BVal_Unknown
          | SOME mmap' => BVal_Mem aty vty mmap'
        else BVal_Unknown))``,
@@ -381,16 +395,21 @@ let
       (type_of_bir_imm a <> ta) ==>
       (bir_eval_store (BVal_Mem ta tv mmap) (BVal_Imm a) en v = BVal_Unknown)) /\
       (!i tv.
-      (type_of_bir_imm i <> tv) ==> (bir_number_of_mem_splits tv (type_of_bir_imm i) <> NONE) ==>
+      (type_of_bir_imm i <> tv) ==> (bir_number_of_mem_splits tv (type_of_bir_imm i) ta <> NONE) ==>
       (bir_eval_store (BVal_Mem ta tv mmap) a BEnd_NoEndian (BVal_Imm i) = BVal_Unknown)) /\
       (!i tv.
-      (bir_number_of_mem_splits tv (type_of_bir_imm i) = NONE) ==>
+      (bir_number_of_mem_splits tv (type_of_bir_imm i) ta = NONE) ==>
       (bir_eval_store (BVal_Mem ta tv mmap) a en (BVal_Imm i) = BVal_Unknown))``,
    SIMP_TAC std_ss [bir_eval_store_Unknown_REWRS])
 
-  val thm_prune1 = SIMP_RULE (std_ss ++ bir_imm_ss ++ DatatypeSimps.expand_type_quants_ss [``:bir_immtype_t``, ``:bir_imm_t``]) [bir_number_of_mem_splits_REWRS, type_of_bir_imm_def] thm_prune0
+  val thm_prune1 = SIMP_RULE (std_ss ++ bir_imm_ss ++ DatatypeSimps.expand_type_quants_ss [``:bir_immtype_t``, ``:bir_imm_t``]) [bir_number_of_mem_splits_REWRS, type_of_bir_imm_def, FORALL_AND_THM] thm_prune0
 
-  val thm_prune2 = SIMP_RULE std_ss [FORALL_AND_THM, GSYM CONJ_ASSOC] (GEN_ALL thm_prune1)
+  val (l1, l2) = partition (is_imp_only o snd o strip_forall o concl) (CONJUNCTS thm_prune1)
+
+  val l1' = map (SIMP_RULE (list_ss++bir_imm_ss++DatatypeSimps.expand_type_quants_ss [``:bir_immtype_t``]) [bir_number_of_mem_splits_REWRS] o (Q.GEN `ta`)) l1
+
+  val thm_prune2 = SIMP_RULE std_ss [FORALL_AND_THM, GSYM CONJ_ASSOC] (GEN_ALL
+    (LIST_CONJ (l1' @ l2)))
 
 
   val thm0 = SIMP_RULE (std_ss) [bir_eval_store_Unknown_REWRS, FORALL_AND_THM] bir_eval_store_BASIC_REWR
